

Department of Mathematics & Computing
Engineering Mathematics I
Tutorial Sheet-IV (Solution)
(Vector Differential and Integral Calculus)

1. Solution: Let $x = \sin t$ then $y = 1 - 2\sin^2 t = \cos 2t$, $\frac{-\pi}{2} \leq t \leq \frac{\pi}{2}$
Hence the parametric form is
 $r(t) = \sin t \mathbf{i} + \cos 2t \mathbf{j}$, $\frac{-\pi}{2} \leq t \leq \frac{\pi}{2}$.
2. Solution: The position vector of a point on the curve is $r(t) = \cos t \mathbf{i} + \sin t \mathbf{j} + t \mathbf{k}$.
Therefore the tangent vector is $r'(t) = -\sin t \mathbf{i} + \cos t \mathbf{j} + \mathbf{k}$
3. Solution: $\vec{F}(1, 1) = 2\mathbf{j}$, $\vec{F}(-1, 0) = -\mathbf{i} - \mathbf{j}$
4. Solution: For this problem lets solve for z to get $z = \frac{15}{4} - \frac{7x}{4} - \frac{3y}{4}$.
The parametric equation for the plane is $\vec{r}(x, y) = \langle x, y, \frac{15}{4} - \frac{7}{4}x - \frac{3}{4}y \rangle$.
5. Solution: $r'(t) = -a \sin t \mathbf{i} + a \cos t \mathbf{j} + c \mathbf{k}$.
6. Solution: $r(t) = (\cos t + \sin t) \mathbf{i} + (\sin t - \cos t) \mathbf{j} + t \mathbf{k}$,
 $r'(t) = (-\sin t + \cos t) \mathbf{i} + (\cos t + \sin t) \mathbf{j} + \mathbf{k}$,
 $r''(t) = (-\cos t - \sin t) \mathbf{i} + (-\sin t + \cos t) \mathbf{j}$,
Hence velocity $v(t) = r'(t)$
 $v(t) = (-\sin t + \cos t) \mathbf{i} + (\cos t + \sin t) \mathbf{j} + \mathbf{k}$,
speed $= |v(t)| = \sqrt{3}$,
acceleration $a(t) = r''(t)$,
 $a(t) = (-\cos t - \sin t) \mathbf{i} + (-\sin t + \cos t) \mathbf{j}$.
7. Solution: $\mathbf{r} = x\mathbf{i} + y\mathbf{j} + z\mathbf{k} \Rightarrow |r| = \sqrt{x^2 + y^2 + z^2}$.
 $\ln |r| = \frac{1}{2} \ln(x^2 + y^2 + z^2)$

$$\begin{aligned}
 \nabla \phi &= \frac{1}{2} \nabla \ln(x^2 + y^2 + z^2) \\
 &= \frac{1}{2} \left\{ \mathbf{i} \frac{2x}{x^2 + y^2 + z^2} + \mathbf{j} \frac{2y}{x^2 + y^2 + z^2} + \mathbf{k} \frac{2z}{x^2 + y^2 + z^2} \right\} \\
 &= \frac{\mathbf{r}}{x^2 + y^2 + z^2} \\
 &= \frac{\mathbf{r}}{r^2}.
 \end{aligned}$$

8. Solution: Let $\phi = \nabla(x \sin(yz) + y \sin(xz) + z \sin(xy))$.

Then

$$\begin{aligned}\nabla\phi &= \mathbf{i}\frac{\partial\phi}{\partial x} + \mathbf{j}\frac{\partial\phi}{\partial y} + \mathbf{k}\frac{\partial\phi}{\partial z} \\ &= \{\sin(yz) + y \cos(xz)z + z \cos(xy)y\}\mathbf{i} + \{x \cos(yz)z + x \sin(xz) + z \cos(xy)x\}\mathbf{j} \\ &\quad + \{\sin(xy) + x \cos(yz)y + y \cos(xz)x\}\mathbf{k} \\ &= \left(\frac{\pi + \sqrt{2}}{2}\right)\mathbf{i}, \quad \text{at}(0, \frac{\pi}{4}, 1).\end{aligned}$$

9. Solution: Let $f(x, y, z) = x^2 + 2y^2 + z^2 - 4$.

$$\text{Now, } \nabla f = \mathbf{i}\frac{\partial f}{\partial x} + \mathbf{j}\frac{\partial f}{\partial y} + \mathbf{k}\frac{\partial f}{\partial z} = 2x\mathbf{i} + 4y\mathbf{j} + 2z\mathbf{k}.$$

The normal vector at $(1, 1, 1)$ is $(\nabla f)_{at(1,1,1)} = 2\mathbf{i} + 4\mathbf{j} + 2\mathbf{k}$.

The unit normal vector at $(1, 1, 1) = \frac{2\mathbf{i}+4\mathbf{j}+2\mathbf{k}}{\sqrt{4+16+4}} = \frac{\mathbf{i}+2\mathbf{j}+\mathbf{k}}{\sqrt{6}}$.

10. Solution:

$$\begin{aligned}RHS &= (g\nabla f - f\nabla g)^2 \\ &= \frac{[g\{\mathbf{i}\frac{\partial f}{\partial x} + \mathbf{j}\frac{\partial f}{\partial y} + \mathbf{k}\frac{\partial f}{\partial z}\} - f(\mathbf{i}\frac{\partial g}{\partial x} + \mathbf{j}\frac{\partial g}{\partial y} + \mathbf{k}\frac{\partial g}{\partial z})]}{g^2} \\ &= \nabla(f/g) = LHS.\end{aligned}$$

11. Solution: $\nabla\phi = (2xyz - 4yz^2)\mathbf{i} + (x^2z - 4xz^2)\mathbf{j} + (x^2y - 8xyz)\mathbf{k}$.

At $(1, 3, 1)$, $\nabla\phi = -6\mathbf{i} - 3\mathbf{j} - 21\mathbf{k}$.

The unit vector in the direction of $2\mathbf{i} - \mathbf{j} - 2\mathbf{k}$ is

$$\hat{b} = \frac{2\mathbf{i} - \mathbf{j} - 2\mathbf{k}}{\sqrt{4+1+4}} = \frac{2}{3}\mathbf{i} - \frac{1}{3}\mathbf{j} - \frac{2}{3}\mathbf{k}.$$

Thus the required directional derivative is, $(\nabla\phi)_{at(1,3,1)} \cdot \hat{b} = 11$

12. Solution: Let $\phi = 2x^2 + y^2 + z^2$.

$$\nabla\phi = 4x\mathbf{i} + 2y\mathbf{j} + 2z\mathbf{k}$$

$$(\nabla\phi)_{at(1,2,3)} = 4\mathbf{i} + 4\mathbf{j} + 6\mathbf{k}$$

Vector form of the line $\frac{x}{3} = \frac{y}{4} = \frac{z}{5}$ is $3k\mathbf{i} + 4k\mathbf{j} + 5k\mathbf{k}$.

The unit vector in the direction of $3k\mathbf{i} + 4k\mathbf{j} + 5k\mathbf{k}$ is,

$$\hat{b} = \frac{3k\mathbf{i} + 4k\mathbf{j} + 5k\mathbf{k}}{\sqrt{9k^2 + 16k^2 + 25k^2}} = \frac{3\mathbf{i} + 4\mathbf{j} + 5\mathbf{k}}{5\sqrt{2}}.$$

Thus the required directional derivative is, $(\nabla\phi)_{at(1,2,3)} \cdot \hat{b} = \frac{58}{5\sqrt{2}}$.

13. Solution: $\nabla\phi = 2z\mathbf{i} - 2y\mathbf{j} + 2x\mathbf{k}$.

The directional derivative is maximum in the direction $(\nabla\phi)_{at (1,3,2)} = 4\mathbf{i} - 6\mathbf{j} + 2\mathbf{k}$.

The magnitude of this maximum is $|(\nabla\phi)_{at (1,3,2)}| = 2\sqrt{14}$.

14. Solution: $\nabla f(x, y) = (2x - y)\mathbf{i} + (-x - 1 + 2y)\mathbf{j}$.

At (x_1, y_1) , $\nabla f(x_1, y_1) = (2x_1 - y_1)\mathbf{i} + (-x_1 - 1 + 2y_1)\mathbf{j}$.

The unit vector in the direction of $\frac{(\mathbf{i} + \sqrt{3}\mathbf{j})}{2}$ is $\frac{(\mathbf{i} + \sqrt{3}\mathbf{j})}{2}$.

Now, the directional derivative $(2x_1 - y_1)\frac{1}{2} + (-x_1 - 1 + 2y_1)\frac{\sqrt{3}}{2} = 0$

$\Rightarrow (2 - \sqrt{3})x_1 + (2\sqrt{3} - 1)y_1 = \sqrt{3}$. Hence the required points are all the points on the line

$$(2 - \sqrt{3})x + (2\sqrt{3} - 1)y = \sqrt{3}$$

15. Solution:

$$\begin{aligned}\nabla \cdot (\bar{r}/r) &= r^{-1}\nabla \cdot \bar{r} + \bar{r} \cdot \nabla r^{-1} \\ &= 3r^{-1} + \bar{r} \cdot (-r^{-1-2}\bar{r}) \quad (\because \nabla r^n = nr^{n-2}\bar{r}) \\ &= 3r^{-1} - r^{-3}\bar{r} \cdot \bar{r} \\ &= 3r^{-1} - r^{-3}r^2 = 2r^{-1}\end{aligned}$$

$$\text{So } \nabla \cdot (\bar{r}/r) = 2\nabla r^{-1}$$

$$= 2(-1)r^{-1-2}\bar{r} = -2r^{-3}\bar{r}.$$

16. Solution:

$$\nabla \cdot \bar{A} = 0$$

$$\begin{aligned}\left(\mathbf{i}\frac{\partial}{\partial x} + \mathbf{j}\frac{\partial}{\partial y} + \mathbf{k}\frac{\partial}{\partial z}\right) \left((bx^2y + yz)\mathbf{i} + (xy^2 - xz^2)\mathbf{j} + (2xyz - 2x^2y^2)\mathbf{k}\right) &= 0 \\ 2bxy + 2xy + 2xy &= 0 \\ b &= -2.\end{aligned}$$

17. Solution:

$$\begin{aligned}\text{Let } f &= \nabla \cdot \bar{U} = \left(\mathbf{i}\frac{\partial}{\partial x} + \mathbf{j}\frac{\partial}{\partial y} + \mathbf{k}\frac{\partial}{\partial z}\right) \left(\frac{x^2z}{2}\mathbf{i} + yx\mathbf{j} + \frac{z^2}{2}\mathbf{k}\right) \\ \nabla f|_{(4,4,2)} &= z\mathbf{i} + \mathbf{k}|_{(4,4,2)} = 2\mathbf{i} + \mathbf{k}\end{aligned}$$

Normal to the sphere $g = x^2 + y^2 + z^2 = 36$ is

$$\begin{aligned}\nabla g|_{(4,4,2)} &= 2(x\mathbf{i} + y\mathbf{j} + z\mathbf{k})|_{(4,4,2)} = 4(2\mathbf{i} + 2\mathbf{j} + \mathbf{k}) \\ \bar{a} = \text{unit normal} &= \frac{\nabla g}{|\nabla g|} = \frac{4(2\mathbf{i} + 2\mathbf{j} + \mathbf{k})}{\sqrt{64 + 64 + 16}} = \frac{2\mathbf{i} + 2\mathbf{j} + \mathbf{k}}{3}\end{aligned}$$

The required directional derivative is

$$\nabla f \cdot \bar{a} = (2\mathbf{i} + \mathbf{k}) \cdot \left(\frac{2\mathbf{i} + 2\mathbf{j} + \mathbf{k}}{3}\right) = \frac{5}{3}.$$

18. Solution:

$$\begin{aligned}\nabla \times \bar{A} &= \begin{vmatrix} \mathbf{i} & \mathbf{j} & \mathbf{k} \\ \frac{\partial}{\partial x} & \frac{\partial}{\partial y} & \frac{\partial}{\partial z} \\ x^2 - yz & y^2 - zx & z^2 - xy \end{vmatrix} \\ &= \mathbf{i}(-x + x) - \mathbf{j}(-y + y) + \mathbf{k}(-z + z) \\ \nabla \times \bar{A} &= 0.\end{aligned}$$

To find f : $\bar{A} = \nabla f = \mathbf{i} \frac{\partial f}{\partial x} + \mathbf{j} \frac{\partial f}{\partial y} + \mathbf{k} \frac{\partial f}{\partial z}$

Comparing components of $\mathbf{i}, \mathbf{j}, \mathbf{k}$, we get

$$\frac{\partial f}{\partial x} = x^2 - yz \quad (1)$$

$$\frac{\partial f}{\partial y} = y^2 - zx \quad (2)$$

$$\frac{\partial f}{\partial z} = z^2 - xy \quad (3)$$

Integrating (1) partially w.r.t x , we get

$$f = \frac{x^3}{3} - xyz + c_1(y, z) \quad (4)$$

Differentiating (4) partially w.r.t y and equating it with (2), we get

$$\frac{\partial c_1}{\partial y} = y^2 \quad (5)$$

Integrating (5) partially w.r.t y

$$c_1(y, z) = \frac{y^3}{3} + c_2(z) \quad (6)$$

Substituting (6) in (4)

$$f = \frac{x^3}{3} - xyz + \frac{y^3}{3} + c_2(z) \quad (7)$$

Differentiating (7) partially w.r.t z and equating it with (3), we get

$$\frac{\partial c_2}{\partial z} = z^2$$

$$c_2(z) = \frac{z^3}{3}$$

$$\text{that is, } f = \frac{x^3 + y^3 + z^3}{3} - xyz.$$

19. Solution: $\vec{F} d\vec{r} = 3xy\mathbf{i} - y^2\mathbf{j}$, $d\vec{r} = dx \mathbf{i} + dy \mathbf{j}$

Also, $y = 2x^2 \Rightarrow dy = 4xdx$

$$\begin{aligned}\text{Now, } \int_C \vec{F} d\vec{r} &= \int_C 3xydx - y^2dy = \int_{x=0}^1 3x.2x^2dx - 4x^4.4xdx \\ &= \left[6x^4/4 - 16x^6/6 \right]_0^1 = -\frac{7}{6}\end{aligned}$$

20. Solution: Like above, $\int_C \vec{F} d\vec{r} = \int_C (x + y^2)dx + (x^2 - y^2)dy$
 $= \int_0^1 (x + x^{4/3})dx + (y^3 - y)dy + \int_0^1 (x + x^2)dx + (x^2 - x)dx = \int_0^1 (x^{4/3}dx + y^3 dy) + \int_0^1 2x^2 dx$
 $= 1/84$

21. Solution: Since C is not closed, so close up the curve C by line segment C' from $(1,1)$ to $(-1,1)$.

Now, $\int_C \vec{F} d\vec{r} = \int (1 + xy^2)dx - x^2 y dy$

$\therefore P = 1 + xy^2, Q = -x^2 y \Rightarrow \delta\theta/\delta x = -2xy, \delta P/\delta y = 2xy$

Applying Green's theorem to the region D , we have,

$$\begin{aligned} \int_{C \cup C'} (1 + xy^2)dx - x^2 y dy &= \int_D \int (-2xy - 2xy) dA = \int_D \int -4xy dA \\ &= \int_{-1}^1 \int_2^1 -4xy dy dx = 0. \end{aligned}$$

22. Solution: $P = x^2 y, Q = -xy^2 \Rightarrow \frac{\delta Q}{\delta x} = -y^2, \frac{\delta P}{\delta y} = x^2$

Now, $\int_C P dx + Q dy = \int_D \int -y^2 - x^2 dA = - \int_D \int (x^2 + y^2) dA = \int_0^{2\pi} \int_0^2 r^2 \cdot r dr d\theta$
 $\Rightarrow - \int_0^{2\pi} \int_0^2 r^3 dr d\theta = - \int_0^{2\pi} \left[\frac{r^4}{4} \right]_0^2 d\theta = - \int_0^{2\pi} 4 d\theta = -8\pi.$

23. Solution: The integral would be $f(x, y, g(x, y))\sqrt{1 + (\delta t/\delta x)^2 + (\delta z/\delta y)^2} dA$

Now $z^2 = 1 - x^2 - y^2 \Rightarrow \delta z/\delta x = -x/z, \delta z/\delta y = -y/z$

Substituting in 2nd equation, we get

$$\begin{aligned} \int_R \int x^2 y^2 z \sqrt{1 + x^2/z^2 + y^2/z^2} dA &= \int_R \int x^2 y^2 \sqrt{1 + x^2 + y^2} dA \\ &= \int_R \int x^2 y^2 dA = \int_{\theta=0}^{2\pi} \int_{r=0}^1 r^2 \cos^2 \theta r^2 \sin^2 \theta r dr d\theta = \pi/24. \end{aligned}$$

24. Solution:

$$\begin{aligned} I &= \int_0^a \int_0^a \int_0^a (x^2 + y^2 + z^2) dx dy dz \\ &= \int_0^a \int_0^a \left[x^2 z + y^2 z + \frac{z^3}{3} \right]_0^a dx dy \\ &= \int_0^a \int_0^a \left[x^2 a + y^2 a + \frac{a^3}{3} \right] dx dy \\ &= \int_0^a \left[x^2 a y + \frac{1}{3} y^3 a + \frac{a^3 y}{3} \right]_0^a dx \\ &= \int_0^a \left(x^2 a^2 + \frac{1}{3} a^4 + \frac{a^4}{3} \right) dx \\ &= a^5 \end{aligned}$$

25. Solution:

$$\begin{aligned}
 I &= \int_{x=0}^2 \int_{y=0}^2 \int_{z=0}^{4-x^2} (2x+y) dx dy dz \\
 &= \int_{x=0}^2 \int_{y=0}^2 (2x+y) (4-x^2) dx dy \\
 &= \int_{x=0}^2 [16x - 4x^3 + 2(4-x^2)] dx \\
 &= \frac{80}{3}
 \end{aligned}$$

26. Solution:

$$\begin{aligned}
 I &= \int_{x=0}^a \int_0^{a-x} \int_0^{a-x-y} x^2 dx dy dz \\
 &= \int_{x=0}^a \int_0^{a-x} x^2 (a-x-y) dx dy \\
 &= \int_{x=0}^a \frac{1}{2} x^2 (a-x)^2 dx = \frac{a^5}{60}
 \end{aligned}$$

27. Solution: By divergence theorem, $\int_S \mathbf{v} \cdot \mathbf{n} dA = \int_D \int \int (\nabla \cdot \mathbf{v}) dV$ and we can find $\nabla \cdot \mathbf{v} = 5y + 3$.

Now,

$$\begin{aligned}
 \int \int \int_D (\nabla \cdot \mathbf{v}) dV &= \int_0^4 \int_0^4 \int_0^{4-x} (5y+3) dy dx dz \\
 &= 4 \int_0^4 \int_0^{4-x} (5y+3) dy dx \\
 &= 4 \int_0^4 \left[\frac{5}{2} y^2 + 3y \right]_0^{4-x} dx \\
 &= 4 \int_0^4 \left[\frac{5}{2} (4-x)^2 + 3(4-x) \right] dx \\
 &= \frac{928}{3}.
 \end{aligned}$$

28. Solution: We have $\nabla \cdot \mathbf{v} = 2x + 4y + 6z$. Therefore,

$$\begin{aligned} \int \int \int_D (\nabla \cdot \mathbf{v}) dV &= \int_0^3 \int_{-3}^3 \int_{y=-\sqrt{9-x^2}}^{y=\sqrt{9-x^2}} (2x + 4y + 6z) dy dx dz \\ &= \int_{-3}^3 \int_{y=-\sqrt{9-x^2}}^{y=\sqrt{9-x^2}} (6x + 12y + 27) dy dx. \end{aligned}$$

Since, x, y are odd functions, we find

$$\begin{aligned} \int \int \int_D (\nabla \cdot \mathbf{v}) dV &= \int_{-3}^3 \int_{y=-\sqrt{9-x^2}}^{y=\sqrt{9-x^2}} 27 dy dx \\ &= 4 \times 27 \int_0^3 \int_0^{\sqrt{9-x^2}} dy dx \\ &= 4 \times 27 \int_0^3 [y]_0^{\sqrt{9-x^2}} dx \\ &= 4 \times 27 \int_0^3 \sqrt{9-x^2} dx \\ &= 4 \times 27 \left[\frac{x}{2} \sqrt{9-x^2} + \frac{9}{2} \sin^{-1} \left(\frac{x}{3} \right) \right]_0^3 \\ &= 9 \times 27 \times \pi = 243\pi. \end{aligned}$$

The surface consists of three parts, S_1 (top), S_2 (bottom) and S_3 (vertical).

On $S_1 : z = 3, \mathbf{n} = \mathbf{k}$.

$$\int \int_{S_1} (\mathbf{v} \cdot \mathbf{n}) dA = 3 \int \int_{S_1} z^2 dA = 243\pi$$

On $S_2 : z = 0, \mathbf{n} = -\mathbf{k}$.

$$\int \int_{S_2} (\mathbf{v} \cdot \mathbf{n}) dA = -3 \int \int_{S_2} z^2 dA = 0$$

On $S_3 : x^2 + y^2 = 9, \mathbf{n} = \frac{2x\mathbf{i} + 2y\mathbf{j}}{2\sqrt{x^2 + y^2}} = \frac{1}{3}(x\mathbf{i} + y\mathbf{j})$

$$\int \int_{S_3} (\mathbf{v} \cdot \mathbf{n}) dA = \frac{1}{3} \int \int_{S_3} (x^3 + 2y^3) dA.$$

By using the cylindrical coordinates, we write $x = 3 \cos \theta, y = 3 \sin \theta, dA = 3d\theta dz$.

$$\begin{aligned} \int \int_{S_3} (\mathbf{v} \cdot \mathbf{n}) dA &= \int_0^3 \int_0^{2\pi} (27 \cos^3 \theta + 54 \sin^3 \theta) d\theta dz \\ &= 27 \int_0^3 \int_0^{2\pi} \left[\left(\frac{3}{4} \cos \theta + \cos 3\theta \right) + 2 \left(\frac{3}{4} \sin \theta + \sin 3\theta \right) \right] d\theta dz = 0 \end{aligned}$$

Thus, $\int_S (\mathbf{v} \cdot \mathbf{n}) dA = \int_D \int (\nabla \cdot \mathbf{v}) dV$.

29. Solution: Applying Stokes's theorem, the given integral can be reduced to

$$\frac{1}{2} \int_C ((y^2 + z^2)dx + (x^2 + z^2)dy + (x^2 + y^2)dz),$$

where C is the curve $x^2 + y^2 - 2ax = 0, z = 0$ or $(x - a)^2 + y^2 = a^2, z = 0$.

Put $x = a(1 + \cos \theta), y = a \sin \theta, z = 0$.

$$\begin{aligned} & \frac{1}{2} \int_C ((y^2 + z^2)dx + (x^2 + z^2)dy + (x^2 + y^2)dz) \\ &= \frac{1}{2} \int_{-\pi}^{\pi} (a^2 \sin^2 \theta (-a \sin \theta) + a^2(1 + \cos \theta)a \cos \theta) d\theta \\ &= \pi a^3. \end{aligned}$$

30. Solution: Consider the projection of S on $x - y$ plane. The projection is the circular region

$x^2 + y^2 \leq 16, z = 0$ and the bounding curve C is the circle $z = 0, x^2 + y^2 = 16$. We have,

$$\int_C \mathbf{v} \cdot d\mathbf{r} = \int_C ((3x - y)dx - 2yz^2 dy - 2y^2 z dz) = \int_C (3x - y)dx$$

since $z = 0$. Take $x = 4 \cos \theta, y = 4 \sin \theta$, we obtain

$$\begin{aligned} \int_C (3x - y)dx &= \int_0^{2\pi} 4(3 \cos \theta - \sin \theta)(-4 \sin \theta) d\theta = -16 \int_0^{2\pi} \left[\frac{3}{2} \sin 2\theta - \frac{1}{2} (1 - \cos 2\theta) \right] d\theta \\ &= 16\pi. \end{aligned}$$

Now, $\nabla \times \mathbf{v} = \mathbf{k}, \mathbf{n} = \frac{2(xi+yj+zk)}{2\sqrt{x^2+y^2+z^2}} = \frac{xi+yj+zk}{4}$ and $(\nabla \times \mathbf{v}) \cdot \mathbf{n} = \frac{z}{4}$. Therefore,

$$\int_S (\nabla \times \mathbf{v}) \cdot \mathbf{n} dA = \int_S \frac{z}{4} dA = \int_R \int \frac{z}{4} \frac{dxdy}{\mathbf{n} \cdot \mathbf{k}} = \int_R \int \frac{z}{4} \frac{dxdy}{z/4} = \int_R \int dxdy = 16\pi$$

which is the area of the circular region in the $x - y$ plane. Hence, Stokes's theorem is proved.